prime number lemma

ch4_euclid_theorem.sml
@@ -8,9 +8,7 @@ g `!x. x divides 0`;
 e (ARW_TAC [divides] THEN EXISTS_TAC ``0`` THEN ARW_TAC[]);
 val DIVIDES_0 = top_thm();
 
-g `!x. 0 divides x = (x=0)`;
-e (ARW_TAC [divides]);
-val DIVIDES_ZERO = top_thm();
+val DIVIDES_ZERO = store_thm("DIVIDES_ZERO",``!x. 0 divides x = (x=0)``,ARW_TAC [divides]);
 
 g `!x. x divides 1 = (x=1)`;
 e (ARW_TAC [divides]);
@@ -59,3 +57,14 @@ val DIVIDES_FACT = store_thm ("DIVIDES_FACT", ``!m n. 0 < m /\ m <=n ==> m divid
 val lemma=store_thm ( "lemma", ``!m. 0 < m ==> ?k. m = SUC k``, Cases THEN ARW_TAC []);
 
 val DIVIDES_FACT = store_thm ("DIVIDES_FACT", ``!m n. 0 < m /\ m <=n ==> m divides (FACT n)``, Induct_on `n-m` THEN REPEAT STRIP_TAC THENL [`m=n` by DECIDE_TAC, ALL_TAC] THEN ARW_TAC [] THENL [ `?k. m = SUC k` by PROVE_TAC [lemma] THEN ARW_TAC [FACT,DIVIDES_LMUL, DIVIDES_REFL], ALL_TAC] THEN `0 < n` by DECIDE_TAC THEN `?k. n = SUC k` by PROVE_TAC [lemma] THEN ARW_TAC [FACT,DIVIDES_RMUL,DIVIDES_REFL]);
+
+(* Prime Number Lemma *)
+val prime = Define `prime p = ~(p=1) /\ !x. x divides p ==> (x=1) \/ (x=p)`;
+
+val NOT_PRIME_0 = store_thm("NOT_PRIME_0", ``~prime 0``, ARW_TAC [prime,DIVIDES_0]);
+
+val NOT_PRIME_1 = store_thm("NOT_PRIME_1", ``~prime 1``, ARW_TAC [prime]);
+
+val PRIME_2 = store_thm("PRIME_2", ``prime 2``, ARW_TAC [prime] THEN PROVE_TAC [ DIVIDES_LE , DIVIDES_ZERO, DECIDE ``~(2=1)``, DECIDE ``~(2=0)``, DECIDE `` x<=2 = (x=0) \/ (x=1) \/ (x=2)``]);
+
+val PRIME_POS = store_thm("PRIME_POS", ``!p. prime p ==> 0<p``, Cases THEN ARW_TAC[NOT_PRIME_0]);
